add stpd2 constructors

dev2015/fsub2.v
@@ -306,15 +306,15 @@ Does it make a difference? It seems like we can always widen f?
 
 
 Inductive stp2: bool -> venv -> ty -> venv -> ty -> list (id*(venv*ty)) -> nat -> Prop :=
-| stp2_topx: forall G1 GH n1,
-    stp2 true G1 TTop G1 TTop GH n1
-| stp2_botx: forall G1 GH n1,
-    stp2 true G1 TBot G1 TBot GH n1
+| stp2_topx: forall G1 G2 GH n1,
+    stp2 true G1 TTop G2 TTop GH n1
+| stp2_botx: forall G1 G2 GH n1,
+    stp2 true G1 TBot G2 TBot GH n1
 | stp2_top: forall G1 G2 GH T n1,
-    stp2 true G1 T G1 T GH n1 ->
+    stp2 false G1 T G1 T GH n1 ->
     stp2 true G1 T G2 TTop GH (S n1)
 | stp2_bot: forall G1 G2 GH T n1,
-    stp2 true G2 T G2 T GH n1 ->
+    stp2 false G2 T G2 T GH n1 ->
     stp2 true G1 TBot G2 T GH (S n1)
 | stp2_bool: forall G1 G2 GH n1,
     stp2 true G1 TBool G2 TBool GH n1
@@ -369,15 +369,116 @@ Inductive stp2: bool -> venv -> ty -> venv -> ty -> list (id*(venv*ty)) -> nat -
     stp2 false G1 (open (TSelH (length GH)) T2) G2 (open (TSelH (length GH)) T4) ((0,(G2, T3))::GH) n2 ->
     stp2 true G1 (TAll T1 T2) G2 (TAll T3 T4) GH (S (n1+n2))
 
-| stp_transf: forall G1 G2 G3 T1 T2 T3 GH n1 n2,
+| stp2_wrapf: forall G1 G2 T1 T2 GH n1,
+    stp2 true G1 T1 G2 T2 GH n1 ->
+    stp2 false G1 T1 G2 T2 GH (S n1)
+| stp2_transf: forall G1 G2 G3 T1 T2 T3 GH n1 n2,
     stp2 true G1 T1 G2 T2 GH n1 ->
     stp2 false G2 T2 G3 T3 GH n2 ->           
     stp2 false G1 T1 G3 T3 GH (S (n1+n2))
-
-| stp_wrapf: forall G1 G2 T1 T2 GH n1,
-    stp2 true G1 T1 G2 T2 GH n1 ->
-    stp2 false G1 T1 G2 T2 GH (S n1)
 .
+
+Definition stpd2 b G1 T1 G2 T2 GH := exists n, stp2 b G1 T1 G2 T2 GH n.
+
+Ltac ep := match goal with
+             | [ |- stp ?M ?G1 ?T1 ?T2 ?N ] => assert (exists (x:nat), stp M G1 T1 T2 x) as EEX
+           end.
+
+Ltac eu := match goal with
+             | H: stpd2 _ _ _ _ _ _ |- _ => destruct H
+(*             | H: exists n: nat ,  _ |- _  =>
+               destruct H as [e P] *)
+           end.
+
+Hint Constructors stp2.
+Hint Unfold stpd2.
+
+Lemma stpd2_topx: forall G1 G2 GH,
+    stpd2 true G1 TTop G2 TTop GH.
+Proof. intros. exists 0. eauto. Qed.
+Lemma stpd2_botx: forall G1 G2 GH,
+    stpd2 true G1 TBot G2 TBot GH.
+Proof. intros. exists 0. eauto. Qed.
+Lemma stpd2_top: forall G1 G2 GH T,
+    stpd2 false G1 T G1 T GH ->
+    stpd2 true G1 T G2 TTop GH.
+Proof. intros. repeat eu. eauto. Qed.
+Lemma stpd2_bot: forall G1 G2 GH T,
+    stpd2 false G2 T G2 T GH ->
+    stpd2 true G1 TBot G2 T GH.
+Proof. intros. repeat eu. eauto. Qed.
+Lemma stpd2_bool: forall G1 G2 GH,
+    stpd2 true G1 TBool G2 TBool GH.
+Proof. intros. exists 0. eauto. Qed.
+Lemma stpd2_fun: forall G1 G2 GH T11 T12 T21 T22,
+    stpd2 false G2 T21 G1 T11 GH ->
+    stpd2 false G1 T12 G2 T22 GH ->
+    stpd2 true G1 (TFun T11 T12) G2 (TFun T21 T22) GH.
+Proof. intros. repeat eu. eauto. Qed.
+Lemma stpd2_mem: forall G1 G2 GH T11 T12 T21 T22,
+    stpd2 false G2 T21 G1 T11 GH ->
+    stpd2 false G1 T12 G2 T22 GH ->
+    stpd2 true G1 (TMem T11 T12) G2 (TMem T21 T22) GH.
+Proof. intros. repeat eu. eauto. Qed.
+
+Lemma stpd2_sel1: forall G1 G2 GX TX x T2 GH,
+    index x G1 = Some (vty GX TX) ->
+    closed 0 0 TX ->
+    stpd2 false GX TX G2 T2 GH ->
+    stpd2 true G1 (TSel x) G2 T2 GH.
+Proof. intros. repeat eu. eauto. Qed.
+
+Lemma stpd2_sel2: forall G1 G2 GX TX x T1 GH,
+    index x G2 = Some (vty GX TX) ->
+    closed 0 0 TX ->
+    stpd2 false G1 T1 GX TX GH ->
+    stpd2 true G1 T1 G2 (TSel x) GH.
+Proof. intros. repeat eu. eauto. Qed.
+
+Lemma stpd2_sela1: forall G1 G2 GX TX x T2 GH,
+    indexr x GH = Some (GX, TX) ->
+    (* closed 0 x TX -> *)
+    stpd2 false GX TX G2 (TMem TBot T2) GH ->
+    stpd2 true G1 (TSelH x) G2 T2 GH.
+Proof. intros. repeat eu. eauto. Qed.
+
+Lemma stpd2_sela2: forall G1 G2 GX TX x T1 GH,
+    indexr x GH = Some (GX, TX) ->
+    (* closed 0 x TX -> *)
+    stpd2 false GX TX G2 (TMem T1 TTop) GH ->
+    stpd2 true G1 T1 G2 (TSelH x) GH.
+Proof. intros. repeat eu. eauto. Qed.
+
+         
+Lemma stpd2_selax: forall G1 G2 GX TX x GH,
+    indexr x GH = Some (GX, TX) ->
+    indexr x GH = Some (GX, TX) ->
+    stpd2 false GX TX G2 (TMem TBot TTop) GH ->
+    (*closed 0 x TX ->*)
+    stpd2 true G1 (TSelH x) G2 (TSelH x) GH.
+Proof. intros. repeat eu. eauto. Qed.
+
+
+Lemma stpd2_all: forall G1 G2 T1 T2 T3 T4 GH, 
+    stpd2 false G2 T3 G1 T1 GH ->
+    closed 1 (length GH) T2 -> 
+    closed 1 (length GH) T4 -> 
+    stpd2 false G1 (open (TSelH (length GH)) T2) G2 (open (TSelH (length GH)) T4) ((0,(G2, T3))::GH) ->
+    stpd2 true G1 (TAll T1 T2) G2 (TAll T3 T4) GH.
+Proof. intros. repeat eu. eauto. Qed.
+
+Lemma stpd2_wrapf: forall G1 G2 T1 T2 GH,
+    stpd2 true G1 T1 G2 T2 GH ->
+    stpd2 false G1 T1 G2 T2 GH.
+Proof. intros. repeat eu. eauto. Qed.
+Lemma stpd2_transf: forall G1 G2 G3 T1 T2 T3 GH,
+    stpd2 true G1 T1 G2 T2 GH ->
+    stpd2 false G2 T2 G3 T3 GH ->           
+    stpd2 false G1 T1 G3 T3 GH.
+Proof. intros. repeat eu. eauto. Qed.
+
+
+
 
 
 
